FSResource.v
@@ -1,10 +1,13 @@
 Require Import List.
 Require Import String.
 
+Require Import Monad.
 Require Import Resource.
 Require Import FileSystem.
 
 Module FSResource (FS : FileSystem) <: Resource.
-  Definition resource : Type := (FS.file_system * FS.file).
+  Definition resource : Type := FS.file_system.
   Definition class : Type := FS.file.
+
+  Definition RS ( A : Type ) := resource -> (A * resource).
 End FSResource.  
