HttpdInterface.v
@@ -1,6 +1,7 @@
 Require Import List.
 Require Import String.
 
+Require Import Monad.
 Require Import Buffer.
 Require Import Resource.
 
@@ -14,24 +15,27 @@ Module Type Httpd (res: Resource).
   Parameter response : Type.
   Parameter connection : Type.
   Definition DM ( A : Type ) := daemon -> (A * daemon).
-
-  Definition RS ( A : Type ) := res.resource -> (A * res.resource).
+  Instance DM_Monad : Monad DM :=
+    { ret A x := fun d => (x, d);
+      bind A B f x := fun d => match x d with
+                            | (y, d') => f y d'
+                            end }.
   
   (** Callbacks. Used as function pointers in C program. **)
   Definition contentReaderCallback : Type :=
-    res.class -> nat -> nat -> buffer (RS bool).
+    res.class -> nat -> nat -> string -> res.RS (nat * string).
 
   Definition contentReaderFreeCallback : Type :=
-    res.class -> RS unit.
+    res.class -> res.RS unit.
 
   (** Httpd interfaces. **)
   Parameter create_response_from_buffer :
-    nat -> responseMemoryMode -> buffer (DM (option response)).
+    nat -> responseMemoryMode -> string -> DM (option response * string).
   Parameter create_response_from_callback :
     nat -> nat -> contentReaderCallback -> res.resource ->
     contentReaderFreeCallback -> DM (option response).
   Parameter queue_response :
-    connection -> nat -> response -> DM bool.
+    option connection -> nat -> option response -> DM bool.
 
   (** Abstract states. **)
   Parameter response_queue : daemon -> list (connection * nat * response).
@@ -42,9 +46,8 @@ Module Type Httpd (res: Resource).
 
   (** Specifications. **)
   Axiom create_response_from_buffer_spec :
-    forall size mode buf d rd buf' r d',
-      create_response_from_buffer size mode buf = (rd, buf') ->
-      rd d = (r, d') ->
+    forall size mode buf d buf' r d',
+      create_response_from_buffer size mode buf d = ((r, buf'), d') ->
       response_queue d = response_queue d' /\
       buf = buf' /\
       (forall res, r = Some res ->
@@ -65,5 +68,6 @@ Module Type Httpd (res: Resource).
     forall conn status res b d d',
       queue_response conn status res d = (b, d') ->
       (forall r, In r (response_queue d) -> In r (response_queue d')) /\
-      In (conn, status, res) (response_queue d').
+      (forall c r, conn = Some c -> res = Some r ->
+              In (c, status, r) (response_queue d')).
 End Httpd.
