Resource.v
@@ -1,4 +1,8 @@
+Require Import Monad.
+
 Module Type Resource.
   Parameter resource : Type.
   Parameter class : Type.
+  
+  Definition RS ( A : Type ) := resource -> (A * resource).
 End Resource.
