Monad.v
@@ -1,0 +1,14 @@
+Class Monad ( M : Type -> Type ) : Type :=
+  { ret { A : Type } : A -> M A;
+    bind { A B : Type } : (A -> M B) -> M A -> M B }.
+
+Notation "x <- P ; Q" := (bind (fun x => Q) P) (at level 100).
+
+Notation "P >> Q" := (bind (fun _ => Q) P) (at level 100).
+
+Instance Option_Monad : Monad option :=
+  { ret A x := Some x;
+    bind A B f a := match a with
+                    | Some a' => f a'
+                    | None => None
+                    end }.
